theories/F_mu_ref/binary/soundness.v
@@ -2,6 +2,7 @@ From WBLogrel.F_mu_ref.binary Require Export context_refinement.
 From iris.algebra Require Import auth frac agree.
 From iris.proofmode Require Import proofmode.
 From iris.program_logic Require Import adequacy.
+From WBLogrel.program_logic Require Import adequacy.
 From WBLogrel.F_mu_ref.unary Require Import soundness.
 From iris.prelude Require Import options.
 
@@ -13,14 +14,14 @@ Proof. solve_inG. Qed.
 
 Lemma basic_soundness Σ `{soundness_unary_preG Σ, inG Σ (authR cfgUR)}
     e e' τ v thp hp :
-  (∀ `{heapIG Σ, cfgSG Σ, ghost_regG Σ}, ⊢ [] ⊨ e ≤log≤ e' : τ) →
+  (∀ `{heapIG Σ, cfgSG Σ}, ⊢ [] ⊨ e ≤log≤ e' : τ) →
   rtc erased_step ([e], ∅) (of_val v :: thp, hp) →
   (∃ thp' hp' v', rtc erased_step ([e'], ∅) (of_val v' :: thp', hp')).
 Proof.
   intros Hlog Hsteps.
   cut (adequate NotStuck e ∅ (λ _ _, ∃ thp' h v, rtc erased_step ([e'], ∅) (of_val v :: thp', h))).
   { destruct 1; naive_solver. }
-  eapply (wp_adequacy Σ _); iIntros (Hinv ?).
+  eapply (wbwp_adequacy Σ _); iIntros (Hinv ? ?).
   iMod (gen_heap_init (∅: state)) as (Hheap) "[Hh _]".
   iMod (own_alloc (● (to_tpool [e'], ∅)
     ⋅ ◯ ((to_tpool [e'] : tpoolUR, ∅) : cfgUR))) as (γc) "[Hcfg1 Hcfg2]".
@@ -28,22 +29,21 @@ Proof.
   set (Hcfg := CFGSG _ _ γc).
   iMod (inv_alloc specN _ (spec_inv ([e'], ∅)) with "[Hcfg1]") as "#Hcfg".
   { iNext. iExists [e'], ∅. rewrite /to_heap fmap_empty. auto. }
-  set (HeapΣ := (HeapIG Σ Hinv Hheap)).
+  set (HeapΣ := (HeapIG Σ Hinv Hheap _)).
   iExists (λ σ _, gen_heap_interp σ), (λ _, True%I); iFrame.
-  iMod ghost_reg_init as (γ) "Hreg".
-  iApply wp_fupd. iApply wp_wand_r.
+  iApply wbwp_fupd. iApply wbwp_wand_r.
   iSplitL.
-  - iPoseProof ((Hlog _ _ _)) as "Hrel".
+  - iPoseProof ((Hlog _ _)) as "Hrel".
     iSpecialize ("Hrel" $! [] [] with "[]").
     { iSplit.
       - by iExists ([e'], ∅).
-      - by iApply (@interp_env_nil Σ HeapΣ _ []). }
+      - iApply (interp_env_nil []). }
     simpl.
     replace e with e.[env_subst[]] at 2 by by asimpl.
     iModIntro.
-    iApply ("Hrel" $! _ 0 [] with "Hreg").
+    iApply ("Hrel" $! 0 []).
     { rewrite /tpool_mapsto. asimpl. by iFrame. }
-  - iModIntro. iIntros (v1); iDestruct 1 as (v2 M) "(% & Hreg & Hj & #Hinterp)".
+  - iModIntro. iIntros (v1); iDestruct 1 as (v2) "(Hj & #Hinterp)".
     iInv specN as (tp σ) ">[Hown Hsteps]" "Hclose"; iDestruct "Hsteps" as %Hsteps'.
     rewrite /tpool_mapsto /=.
     iDestruct (own_valid_2 with "Hown Hj") as %Hvalid.
@@ -57,11 +57,11 @@ Qed.
 Lemma binary_soundness Σ `{soundness_unary_preG Σ, inG Σ (authR cfgUR)}
     Γ e e' τ :
   (Γ ⊢ₜ e : τ) → (Γ ⊢ₜ e' : τ) →
-  (∀ `{heapIG Σ, cfgSG Σ, ghost_regG Σ}, ⊢ Γ ⊨ e ≤log≤ e' : τ) →
+  (∀ `{heapIG Σ, cfgSG Σ}, ⊢ Γ ⊨ e ≤log≤ e' : τ) →
   Γ ⊨ e ≤ctx≤ e' : τ.
 Proof.
   intros He He' Hlog; repeat split; auto.
-  intros K thp σ v ?. eapply (basic_soundness Σ _)=> ???.
+  intros K thp σ v ?. eapply (basic_soundness Σ _)=> ??.
   iApply (bin_log_related_under_typed_ctx _ _ _ _ []);
     [by eapply typed_n_closed|by eapply typed_n_closed|done|].
   iApply Hlog.
