theories/F_mu_ref/unary/examples/very_awkward.v
@@ -1,7 +1,7 @@
 From iris.algebra Require Import auth gmap.
-From iris.staging.algebra Require Import monotone.
+From iris.unstable.algebra Require Import monotone.
 From iris.proofmode Require Import proofmode.
-From iris.program_logic Require Import lifting adequacy.
+From WBLogrel.program_logic Require Import lifting adequacy.
 From WBLogrel.F_mu_ref Require Import wp_rules.
 From WBLogrel.F_mu_ref.unary Require Import soundness.
 From iris.prelude Require Import options.
@@ -86,7 +86,7 @@ Global Instance sub_relΣ_inG Σ : subG relΣ Σ → inG Σ (authUR (mraUR rel))
 Proof. solve_inG. Qed.
 
 Section very_awkward.
-  Context `{heapIG Σ, ghost_regG Σ}.
+  Context `{!heapIG Σ, !inG Σ (authUR gstackUR)}.
 
   Lemma very_awkward_sem_typed `{!inG Σ (authUR (mraUR rel))} :
     ⊢ [] ⊨ very_awkward_packed :
@@ -95,96 +95,89 @@ Section very_awkward.
     iIntros (? vs) "!# HΔ".
     iDestruct (interp_env_length with "HΔ") as %Hlen; destruct vs; simplify_eq.
     iClear (Hlen) "HΔ". asimpl.
-    iIntros (M) "Hreg /=".
-    iApply (wp_bind (fill [PairLCtx _; PackCtx])).
-    iApply (wp_bind (fill [LetInCtx _])).
-    iApply wp_alloc; first done.
+    iApply (wbwp_bind (fill [PairLCtx _; PackCtx])).
+    iApply (wbwp_bind (fill [LetInCtx _])).
+    iApply wbwp_alloc; first done.
     iNext. iIntros (l) "Hl /=".
-    iApply wp_pure_step_later; auto.
-    iNext. asimpl.
+    iApply wbwp_pure_step_later; auto.
+    iNext; iIntros "_". asimpl.
     iMod (exactly_alloc false) as (γ) "Hex".
-    iMod (res_name_alloc _ γ with "Hreg") as (id HidM) "[Hreg Hid]".
-    rewrite insert_union_singleton_r; last first.
-    { rewrite -(not_elem_of_dom (D := gset ghost_id)); done. }
+    iApply (wbwp_make_gstack _ _ γ); iIntros (n) "Hfrg".
+    iDestruct (gstack_frag_exists with "Hfrg") as "#Hx".
     iMod (inv_alloc
             (nroot .@ "awk") _
-            (∃ γ b, named_ghost id 1 γ ∗ exactly γ b ∗ if b then l ↦ᵢ (#nv 1) else l ↦ᵢ (#nv 0))%I
-            with "[Hex Hid Hl]") as "#Hinv".
-    { iNext; iExists γ, false; iFrame. }
-    iApply wp_value.
+            (∃ γ s b, gstack_frag n s ∗ ⌜gtop s = Some γ⌝ ∗ exactly γ b ∗
+               if b then l ↦ᵢ (#nv 1) else l ↦ᵢ (#nv 0))%I with "[Hex Hfrg Hl]") as "#Hinv".
+    { iNext; iExists γ, _, false; iFrame; rewrite gtop_gsingleton; done. }
+    iApply wbwp_value.
     simpl.
-    iApply wp_value.
-    iExists _; iFrame; iSplit; last first.
-    { iPureIntro. apply map_union_subseteq_l. }
+    iApply wbwp_value.
     iModIntro.
     iExists (PersPred (λ v, ⌜v = (#nv 1)⌝))%I, _; iSplit; first done.
     iExists (LamV _), (LamV _); iSplit; first done.
-    clear M HidM.
     iSplit; last first.
-    { iIntros "!#" (M ?) "Hreg -> /=".
-      iApply wp_pure_step_later; auto; iNext; asimpl.
-      iApply (wp_bind (fill [IfCtx _ _])).
-      iApply wp_pure_step_later; auto; iNext; simpl.
-      iApply wp_value; simpl.
-      iApply wp_pure_step_later; auto; iNext; simpl.
-      iApply wp_value; simpl.
-      iExists _; iFrame; done. }
-    iIntros "!#" (M f) "Hreg #Hf /=".
-    iApply wp_pure_step_later; auto. iNext. asimpl.
-    iApply (wp_bind (fill [SeqCtx _])).
-    iInv (nroot .@ "awk") as (γ1 b) "(>Hid & >Hex1 & Hl)" "Hcl".
+    { iIntros "!#" (?) "-> /=".
+      iApply wbwp_pure_step_later; auto; iNext; iIntros "_"; asimpl.
+      iApply (wbwp_bind (fill [IfCtx _ _])).
+      iApply wbwp_pure_step_later; auto; iNext; iIntros "_"; simpl.
+      iApply wbwp_value; simpl.
+      iApply wbwp_pure_step_later; auto; iNext; iIntros "_"; simpl.
+      iApply wbwp_value; done. }
+    iIntros "!#" (f) "#Hf /=".
+    iApply (wbwp_get_gstack_full n with "[$]"); first done.
+    iIntros (s) "Hfl".
+    iApply wbwp_pure_step_later; auto. iNext; iIntros "_"; asimpl.
+    iApply (wbwp_bind (fill [SeqCtx _])).
+    iInv (nroot .@ "awk") as (γ1 s' b) "(>Hfr & >% & >Hex1 & Hl)" "Hcl".
     iAssert (∃ v, ▷ l ↦ᵢ v)%I with "[Hl]" as (?) ">Hl".
     { destruct b; iExists _; iFrame. }
-    iDestruct (named_ghost_agree with "Hreg Hid") as %Hids1.
+    iDestruct (gstacks_agree with "Hfl Hfr") as %<-.
     iMod (exactly_alloc false) as (γ2) "Hex2".
-    iMod (named_ghost_update _ _ _ γ2 with "Hreg Hid") as "[Hreg Hid]".
-    iApply (wp_store with "[$]").
+    iMod (gstack_push _ _ _ γ2 with "Hfl Hfr") as "[Hfl Hfr]".
+    iApply (wbwp_store with "[$]").
     iNext. iIntros "Hl".
-    iMod ("Hcl" with "[Hex2 Hid Hl]") as "_".
-    { iNext; iExists γ2, false; iFrame. }
+    iMod ("Hcl" with "[Hex2 Hfr Hl]") as "_".
+    { iNext; iExists γ2, _, false; iFrame; rewrite gtop_gpush; done. }
     iModIntro.
-    iApply wp_pure_step_later; auto. iNext.
+    iApply wbwp_pure_step_later; auto. iNext; iIntros "_".
     iMod (exactly_update _ _ true with "Hex1") as "[Hex1 Hat1]"; first done.
-    iApply (wp_bind (fill [SeqCtx _])).
-    iApply (wp_wand with "[Hreg]").
-    { iApply ("Hf" $! _ UnitV with "[$] [//]"). }
-    iIntros (?); iDestruct 1 as (N) "(-> & %HN & Hreg)"; simplify_eq/=.
-    iApply wp_pure_step_later; auto. iNext.
-    iApply (wp_bind (fill [SeqCtx _])).
-    iInv (nroot .@ "awk") as (γ3 b2) "(>Hid & >Hex2 & Hl)" "Hcl".
+    iApply (wbwp_bind (fill [SeqCtx _])).
+    iApply (wbwp_wand with "[Hfl]").
+    { iApply (wbwp_mend with "Hfl").
+      replace ((∅ ∪ {[n]}) ∖ {[n]}) with (∅ : gset ghost_id) by set_solver.
+      iApply ("Hf" $! UnitV); done. }
+    iIntros (?) "[Hfl ->] /=".
+    iApply wbwp_pure_step_later; auto. iNext; iIntros "_".
+    iApply (wbwp_bind (fill [SeqCtx _])).
+    iInv (nroot .@ "awk") as (γ3 s' b2) "(>Hfr & >%Hγ3 & >Hex2 & Hl)" "Hcl".
     iAssert (∃ v, ▷ l ↦ᵢ v)%I with "[Hl]" as (?) ">Hl".
     { destruct b2; iExists _; iFrame. }
-    iMod (named_ghost_update _ _ _ γ1 with "Hreg Hid") as "[Hreg Hid]".
-    iApply (wp_store with "[$]").
+    iDestruct (gstacks_agree with "Hfl Hfr") as %<-.
+    iMod (gstack_pop with "Hfl Hfr") as "[Hfl Hfr]".
+    iApply (wbwp_store with "[$]").
     iNext; iIntros "Hl".
-    iMod ("Hcl" with "[Hex1 Hid Hl]") as "_".
-    { iNext; iExists γ1, true; iFrame. }
+    iMod ("Hcl" with "[Hex1 Hfr Hl]") as "_".
+    { iNext; iExists γ1, _, true; iFrame; done. }
     iModIntro. simpl.
-    iApply wp_pure_step_later; auto. iNext.
-    iApply (wp_bind (fill [SeqCtx _])).
-    iApply (wp_wand with "[Hreg]").
-    { iApply ("Hf" $! _ UnitV with "[$] [//]"). }
-    iIntros (?); iDestruct 1 as (N') "(-> & %HN' & Hreg)"; simplify_eq/=.
-    iApply wp_pure_step_later; auto. iNext.
-    iInv (nroot .@ "awk") as (γ4 b3) "(>Hid & >Hex1 & Hl)" "Hcl".
-    iDestruct (named_ghost_agree with "Hreg Hid") as %Hids2.
-    assert (N' !! id = Some γ1) as Heq.
-    { eapply lookup_weaken; last by apply HN'.
-      rewrite lookup_insert; done. }
+    iApply wbwp_pure_step_later; auto. iNext; iIntros "_".
+    iApply (wbwp_bind (fill [SeqCtx _])).
+    iApply (wbwp_wand with "[Hfl]").
+    { iApply (wbwp_mend with "Hfl").
+      replace ((∅ ∪ {[n]}) ∖ {[n]}) with (∅ : gset ghost_id) by set_solver.
+      iApply ("Hf" $! UnitV); done. }
+    iIntros (?) "[Hfl ->]"; simplify_eq/=.
+    iApply wbwp_pure_step_later; auto. iNext; iIntros "_".
+    iInv (nroot .@ "awk") as (γ4 ? b3) "(>Hfr & >% & >Hex1 & Hl)" "Hcl".
+    iDestruct (gstacks_agree with "Hfl Hfr") as %<-.
     simplify_eq.
     iDestruct (exatly_atleast_rel with "Hex1 Hat1") as %?.
     destruct b3; last done.
-    iApply (wp_load with "[$]").
+    iApply (wbwp_load with "[$]").
     iNext; iIntros "Hl".
-    iMod ("Hcl" with "[Hex1 Hid Hl]") as "_".
-    { iNext; iExists _, true; iFrame. }
+    iMod ("Hcl" with "[Hex1 Hfr Hl]") as "_".
+    { iNext; iExists _, _, true; iFrame; done. }
     iModIntro.
-    iExists _; iFrame.
-    iSplit; first done.
-    iPureIntro.
-    etrans; last apply HN'.
-    etrans; last apply insert_mono, HN.
-    rewrite insert_insert insert_id; auto.
+    iFrame; done.
   Qed.
 
   Lemma very_awkward_self_apply_sem_typed `{!inG Σ (authUR (mraUR rel))} :
@@ -193,56 +186,47 @@ Section very_awkward.
     iIntros (? vs) "!# HΔ".
     iDestruct (interp_env_length with "HΔ") as %Hlen; destruct vs; simplify_eq.
     iClear (Hlen) "HΔ". asimpl.
-    iIntros (M) "Hreg /=".
-    iApply (wp_bind (fill [UnpackInCtx _])).
-    iApply (wp_wand with "[Hreg]").
-    { iApply (very_awkward_sem_typed $! [] []); [iApply interp_env_nil|]; done. }
+    iApply (wbwp_bind (fill [UnpackInCtx _])).
+    iApply wbwp_wand.
+    { iApply (very_awkward_sem_typed $! [] []); iApply interp_env_nil. }
     simpl.
-    iIntros (v). iDestruct 1 as (N) "(#Hv & %HN & Hreg)".
+    iIntros (v) "#Hv".
     iDestruct "Hv" as (τi w) "[-> Hw]".
     iDestruct "Hw" as (f test) "(-> & #Hf & #Htest) /=".
-    iApply wp_pure_step_later; auto. iNext. asimpl.
-    iApply (wp_bind (fill [LetInCtx _])).
-    iApply wp_pure_step_later; auto. iNext.
-    iApply wp_value; simpl.
-    iApply wp_pure_step_later; auto. iNext. asimpl.
-    iApply (wp_bind (fill [LetInCtx _])).
-    iApply wp_pure_step_later; auto. iNext.
-    iApply wp_value; simpl.
-    iApply wp_pure_step_later; auto. iNext. asimpl.
-    iApply (wp_bind (fill [AppRCtx _])).
-    iApply (wp_wand with "[Hreg]").
-    { iApply ("Hf" $! _ (LamV _) with "[$]").
-      iIntros "!#" (N' ?) "Hreg -> /=".
-      iApply wp_pure_step_later; auto. iNext. asimpl.
-      iApply (wp_bind (fill [SeqCtx _])).
-      iApply (wp_wand with "[Hreg]").
-      - iApply ("Hf" $! _ (LamV _) with "[$]").
-        iIntros "!#" (N'' ?) "Hreg -> /=".
-        iApply wp_pure_step_later; auto. iNext. simpl.
-        iApply wp_value; iExists _; iFrame; done.
-      - iIntros (w) "/=". iDestruct 1 as (N'') "(#Hτi & %HN'' & Hreg)".
-        iApply wp_pure_step_later; auto. iNext.
-        iApply wp_value; iExists _; iFrame; done. }
-    iIntros (w) "/=". iDestruct 1 as (N') "(#Hτi & %HN' & Hreg)".
-    iApply (wp_wand with "[Hreg]").
-    { iApply ("Htest" with "[$] [//]"). }
-    iIntros (w') "/=". iDestruct 1 as (N'') "(-> & %HN'' & Hreg)".
-    iExists _; iFrame. iSplit; first done.
-    iPureIntro.
-    etrans; last done.
-    etrans; done.
+    iApply wbwp_pure_step_later; auto. iNext; iIntros "_". asimpl.
+    iApply (wbwp_bind (fill [LetInCtx _])).
+    iApply wbwp_pure_step_later; auto. iNext; iIntros "_".
+    iApply wbwp_value; simpl.
+    iApply wbwp_pure_step_later; auto. iNext; iIntros "_". asimpl.
+    iApply (wbwp_bind (fill [LetInCtx _])).
+    iApply wbwp_pure_step_later; auto. iNext; iIntros "_".
+    iApply wbwp_value; simpl.
+    iApply wbwp_pure_step_later; auto. iNext; iIntros "_". asimpl.
+    iApply (wbwp_bind (fill [AppRCtx _])).
+    iApply wbwp_wand.
+    { iApply ("Hf" $! (LamV _)).
+      iIntros "!#" (?) "-> /=".
+      iApply wbwp_pure_step_later; auto. iNext; iIntros "_". asimpl.
+      iApply (wbwp_bind (fill [SeqCtx _])).
+      iApply wbwp_wand.
+      - iApply ("Hf" $! (LamV _)).
+        iIntros "!#" (?) "-> /=".
+        iApply wbwp_pure_step_later; auto. iNext; iIntros "_". simpl.
+        iApply wbwp_value; done.
+      - iIntros (w) "Hτi /=".
+        iApply wbwp_pure_step_later; auto. iNext; iIntros "_".
+        iApply wbwp_value; done. }
+    iIntros (w) "#Hτi /=".
+    iApply ("Htest" with "[$]").
   Qed.
 
 End very_awkward.
-
-
 
 Theorem very_awkward_self_apply_safe thp σ σ' e' :
   rtc erased_step ([very_awkward_self_apply], σ) (thp, σ') → e' ∈ thp →
   not_stuck e' σ'.
 Proof.
-  set (Σ := #[invΣ ; gen_heapΣ loc val ; ghost_regΣ; relΣ]).
+  set (Σ := #[invΣ ; gen_heapΣ loc val ; gstacksΣ; relΣ]).
   set (HG := soundness_unary_preIG Σ _ _ _).
   apply (soundness Σ _ TUnit).
   intros; apply very_awkward_self_apply_sem_typed.
