theories/F_mu_ref/unary/fundamental.v
@@ -1,22 +1,22 @@
 From iris.base_logic Require Import invariants.
-From iris.program_logic Require Import lifting.
+From WBLogrel.program_logic Require Import lifting.
 From iris.proofmode Require Import proofmode.
 From WBLogrel.F_mu_ref.unary Require Export logrel.
 From WBLogrel.F_mu_ref Require Export wp_rules.
 From iris.prelude Require Import options.
 
-Definition log_typed `{heapIG Σ, ghost_regG Σ} (Γ : list type) (e : expr) (τ : type) : iProp Σ :=
-  □ ∀ Δ vs, ⟦ Γ ⟧* Δ vs -∗ ⟦ τ ⟧ₑ Δ e.[env_subst vs].
+Definition log_typed `{!heapIG Σ, !inG Σ (authUR gstackUR)} (Γ : list type) (e : expr) (τ : type)
+  : iProp Σ := □ ∀ Δ vs, ⟦ Γ ⟧* Δ vs -∗ ⟦ τ ⟧ₑ Δ e.[env_subst vs].
 Notation "Γ ⊨ e : τ" := (log_typed Γ e τ) (at level 74, e, τ at next level).
 
 Section typed_interp.
-  Context `{heapIG Σ, ghost_regG Σ}.
+  Context `{!heapIG Σ}.
   Notation D := (persistent_predO val (iPropI Σ)).
 
-  Local Tactic Notation "smart_wp_bind"
+  Local Tactic Notation "smart_wbwp_bind"
         uconstr(ctx) ident(v) constr(Hv) uconstr(Hp) :=
-    iApply (wp_bind (fill [ctx]));
-    iApply (wp_wand with "[-]"); [iApply Hp; trivial|]; cbn;
+    iApply (wbwp_bind (fill [ctx]));
+    iApply (wbwp_wand with "[-]"); [iApply Hp; trivial|]; cbn;
     iIntros (v) Hv.
 
   Lemma sem_typed_var Γ x τ :
@@ -25,107 +25,72 @@ Section typed_interp.
     iIntros (? Δ vs) "!# #HΓ"; simpl.
     iDestruct (interp_env_Some_l with "HΓ") as (v) "[% ?]"; first done.
     erewrite env_subst_lookup; eauto.
-    iIntros (?) "?"; iApply wp_value; iExists _; iFrame; iSplit; done.
+    iApply wbwp_value; done.
   Qed.
 
   Lemma sem_typed_unit Γ : ⊢ Γ ⊨ Unit : TUnit.
-  Proof.
-    iIntros (Δ vs) "!# #HΓ".
-    iIntros (?) "?"; iApply wp_value; iExists _; iFrame; iSplit; done.
-  Qed.
+  Proof. iIntros (Δ vs) "!# #HΓ". iApply wbwp_value; done. Qed.
 
   Lemma sem_typed_nat Γ n : ⊢ Γ ⊨ #n n : TNat.
-  Proof.
-    iIntros (Δ vs) "!# #HΓ /=".
-    iIntros (?) "?"; iApply wp_value; iExists _; iFrame; iSplit; eauto.
-  Qed.
+  Proof. iIntros (Δ vs) "!# #HΓ /=". iApply wbwp_value; iExists _; done. Qed.
 
   Lemma sem_typed_bool Γ b : ⊢ Γ ⊨ #♭ b : TBool.
-  Proof.
-    iIntros (Δ vs) "!# #HΓ /=".
-    iIntros (?) "?"; iApply wp_value; iExists _; iFrame; iSplit; eauto.
-  Qed.
+  Proof. iIntros (Δ vs) "!# #HΓ /=". iApply wbwp_value; iExists _; done. Qed.
 
   Lemma sem_typed_nat_binop Γ op e1 e2 :
     Γ ⊨ e1 : TNat -∗ Γ ⊨ e2 : TNat -∗ Γ ⊨ BinOp op e1 e2 : binop_res_type op.
   Proof.
     iIntros "#IH1 #IH2" (Δ vs) "!# #HΓ /=".
-    iIntros (?) "?".
-    smart_wp_bind (BinOpLCtx _ e2.[env_subst vs]) v "Hv" "IH1".
-    iDestruct "Hv" as (N1 [] ?) "?".
-    smart_wp_bind (BinOpRCtx _ v) v' "Hv'" "IH2".
-    iDestruct "Hv'" as (N2 [] ?) "?".
+    smart_wbwp_bind (BinOpLCtx _ e2.[env_subst vs]) v "Hv" "IH1".
+    iDestruct "Hv" as (?) "%".
+    smart_wbwp_bind (BinOpRCtx _ v) v' "Hv'" "IH2".
+    iDestruct "Hv'" as (?) "%".
     simplify_eq/=.
-    iApply wp_pure_step_later; auto. iNext. iApply wp_value.
-    iExists _; iSplit; last (iSplit; last (by iFrame); iPureIntro; etrans; done).
+    iApply wbwp_pure_step_later; first done. iNext; iIntros "_". iApply wbwp_value.
     destruct op; simpl; try destruct eq_nat_dec;
       try destruct le_dec; try destruct lt_dec; eauto 10.
   Qed.
 
-  Lemma sem_typed_pair Γ e1 e2 τ1 τ2 :
-    Γ ⊨ e1 : τ1 -∗ Γ ⊨ e2 : τ2 -∗ Γ ⊨ Pair e1 e2 : TProd τ1 τ2.
+  Lemma sem_typed_pair Γ e1 e2 τ1 τ2 : Γ ⊨ e1 : τ1 -∗ Γ ⊨ e2 : τ2 -∗ Γ ⊨ Pair e1 e2 : TProd τ1 τ2.
   Proof.
     iIntros "#IH1 #IH2" (Δ vs) "!# #HΓ"; simpl.
-    iIntros (?) "?".
-    smart_wp_bind (PairLCtx e2.[env_subst vs]) v "Hv" "IH1".
-    iDestruct "Hv" as (N1) "(#?&%&?)".
-    smart_wp_bind (PairRCtx v) v' "Hv'" "IH2".
-    iDestruct "Hv'" as (N2) "(#?&%&?)".
-    iApply wp_value.
-    iExists _; iSplit; last (iSplit; last (by iFrame); iPureIntro; etrans; done).
-    eauto.
+    smart_wbwp_bind (PairLCtx e2.[env_subst vs]) v "#Hv" "IH1".
+    smart_wbwp_bind (PairRCtx v) v' "#Hv'" "IH2".
+    iApply wbwp_value; eauto.
   Qed.
 
-  Lemma sem_typed_fst Γ e τ1 τ2 :
-        Γ ⊨ e : TProd τ1 τ2 -∗ Γ ⊨ Fst e : τ1.
+  Lemma sem_typed_fst Γ e τ1 τ2 : Γ ⊨ e : TProd τ1 τ2 -∗ Γ ⊨ Fst e : τ1.
   Proof.
     iIntros "#IH" (Δ vs) "!# #HΓ"; simpl.
-    iIntros (?) "?".
-    smart_wp_bind (FstCtx) v "Hv" "IH"; cbn.
-    iDestruct "Hv" as (N1) "(#Hv&%&?)".
+    smart_wbwp_bind (FstCtx) v "#Hv" "IH"; cbn.
     iDestruct "Hv" as (w1 w2) "#[% [H2 H3]]"; subst.
     simpl.
-    iApply wp_pure_step_later; auto.
-    iApply wp_value.
-    iExists _; iSplit; last (iSplit; last (by iFrame); iPureIntro; etrans; done).
-    done.
+    iApply wbwp_pure_step_later; auto. iNext; iIntros "_".
+    iApply wbwp_value; done.
   Qed.
 
-  Lemma sem_typed_snd Γ e τ1 τ2 :
-    Γ ⊨ e : TProd τ1 τ2 -∗ Γ ⊨ Snd e : τ2.
+  Lemma sem_typed_snd Γ e τ1 τ2 : Γ ⊨ e : TProd τ1 τ2 -∗ Γ ⊨ Snd e : τ2.
   Proof.
     iIntros "#IH" (Δ vs) "!# #HΓ"; simpl.
-    iIntros (?) "?".
-    smart_wp_bind (SndCtx) v "Hv" "IH"; cbn.
-    iDestruct "Hv" as (N1) "(#Hv&%&?)".
+    smart_wbwp_bind (SndCtx) v "#Hv" "IH"; cbn.
     iDestruct "Hv" as (w1 w2) "#[% [H2 H3]]"; subst.
     simpl.
-    iApply wp_pure_step_later; auto.
-    iApply wp_value.
-    iExists _; iSplit; last (iSplit; last (by iFrame); iPureIntro; etrans; done).
-    done.
+    iApply wbwp_pure_step_later; auto. iNext; iIntros "_".
+    iApply wbwp_value; done.
   Qed.
 
   Lemma sem_typed_injl Γ e τ1 τ2 : Γ ⊨ e : τ1 -∗ Γ ⊨ InjL e : (TSum τ1 τ2).
   Proof.
     iIntros "#IH" (Δ vs) "!# #HΓ"; simpl.
-    iIntros (?) "?".
-    smart_wp_bind (InjLCtx) v "Hv" "IH"; cbn.
-    iDestruct "Hv" as (N1) "(#Hv&%&?)".
-    iApply wp_value.
-    iExists _; iSplit; last (iSplit; last (by iFrame); iPureIntro; etrans; done).
-    eauto.
+    smart_wbwp_bind (InjLCtx) v "#Hv" "IH"; cbn.
+    iApply wbwp_value; eauto.
   Qed.
 
   Lemma sem_typed_injr Γ e τ1 τ2 : Γ ⊨ e : τ2 -∗ Γ ⊨ InjR e : TSum τ1 τ2.
   Proof.
     iIntros "#IH" (Δ vs) "!# #HΓ"; simpl.
-    iIntros (?) "?".
-    smart_wp_bind (InjRCtx) v "Hv" "IH"; cbn.
-    iDestruct "Hv" as (N1) "(#Hv&%&?)".
-    iApply wp_value.
-    iExists _; iSplit; last (iSplit; last (by iFrame); iPureIntro; etrans; done).
-    eauto.
+    smart_wbwp_bind (InjRCtx) v "#Hv" "IH"; cbn.
+    iApply wbwp_value; eauto.
   Qed.
 
   Lemma sem_typed_case Γ e0 e1 e2 τ1 τ2 τ3 :
@@ -135,158 +100,103 @@ Section typed_interp.
     Γ ⊨ Case e0 e1 e2 : τ3.
   Proof.
     iIntros "#IH1 #IH2 #IH3" (Δ vs) "!# #HΓ"; simpl.
-    iIntros (?) "?".
-    smart_wp_bind (CaseCtx _ _) v "Hv" "IH1"; cbn.
-    iDestruct "Hv" as (N1) "(#Hv&%&Hreg)".
+    smart_wbwp_bind (CaseCtx _ _) v "#Hv" "IH1"; cbn.
     iDestruct (interp_env_length with "HΓ") as %?.
     iDestruct "Hv" as "[Hv|Hv]"; iDestruct "Hv" as (w) "[% Hw]"; simplify_eq/=.
-    + iApply wp_pure_step_later; first done. asimpl. iNext.
-      iApply (wp_wand with "[Hreg]"); first
-        iApply ("IH2" $! Δ (w :: vs) with "[] Hreg"); first by iApply interp_env_cons; auto.
-      iIntros (v). iDestruct 1 as (N) "(?&%&?)".
-      iExists _; iFrame; iPureIntro.
-      etrans; done.
-    + iApply wp_pure_step_later; first done. asimpl. iNext.
-      iApply (wp_wand with "[Hreg]"); first
-        iApply ("IH3" $! Δ (w :: vs) with "[] Hreg"); first by iApply interp_env_cons; auto.
-      iIntros (v). iDestruct 1 as (N) "(?&%&?)".
-      iExists _; iFrame; iPureIntro.
-      etrans; done.
+    + iApply wbwp_pure_step_later; first done. asimpl. iNext; iIntros "_".
+      iApply ("IH2" $! Δ (w :: vs) with "[]"); first by iApply interp_env_cons; auto.
+    + iApply wbwp_pure_step_later; first done. asimpl. iNext; iIntros "_".
+      iApply ("IH3" $! Δ (w :: vs) with "[]"); first by iApply interp_env_cons; auto.
   Qed.
 
   Lemma sem_typed_if Γ e0 e1 e2 τ :
     Γ ⊨ e0 : TBool -∗ Γ ⊨ e1 : τ -∗ Γ ⊨ e2 : τ -∗ Γ ⊨ If e0 e1 e2 : τ.
   Proof.
     iIntros "#IH1 #IH2 #IH3" (Δ vs) "!# #HΓ"; simpl.
-    iIntros (?) "?".
-    smart_wp_bind (IfCtx _ _) v "Hv" "IH1"; cbn.
-    iDestruct "Hv" as (N1) "(#Hv&%&Hreg)".
+    smart_wbwp_bind (IfCtx _ _) v "#Hv" "IH1"; cbn.
     iDestruct "Hv" as ([]) "%"; subst; simpl;
-      [iApply wp_pure_step_later .. ]; auto; iNext.
-    - iApply (wp_wand with "[Hreg]"); first
-        iApply ("IH2" with "[] Hreg"); first done.
-      iIntros (v). iDestruct 1 as (N) "(?&%&?)".
-      iExists _; iFrame; iPureIntro.
-      etrans; done.
-    - iApply (wp_wand with "[Hreg]"); first
-        iApply ("IH3" with "[] Hreg"); first done.
-      iIntros (v). iDestruct 1 as (N) "(?&%&?)".
-      iExists _; iFrame; iPureIntro.
-      etrans; done.
+      [iApply wbwp_pure_step_later .. ]; auto; iNext; iIntros "_".
+    - iApply ("IH2" with "[]"); first done.
+    - iApply ("IH3" with "[]"); first done.
   Qed.
 
-  Lemma sem_typed_rec Γ e τ1 τ2 :
-    TArrow τ1 τ2 :: τ1 :: Γ ⊨ e : τ2 -∗ Γ ⊨ Rec e : TArrow τ1 τ2.
+  Lemma sem_typed_rec Γ e τ1 τ2 : TArrow τ1 τ2 :: τ1 :: Γ ⊨ e : τ2 -∗ Γ ⊨ Rec e : TArrow τ1 τ2.
   Proof.
     iIntros "#IH" (Δ vs) "!# #HΓ"; simpl.
-    iIntros (?) "?".
-    iApply wp_value. simpl.
-    iExists _; iFrame; iSplit; last done.
-    iModIntro. iLöb as "IHL". iIntros (M' w) "Hreg #Hw".
+    iApply wbwp_value. simpl.
+    iModIntro. iLöb as "IHL". iIntros (w) "#Hw".
     iDestruct (interp_env_length with "HΓ") as %?.
-    iApply wp_pure_step_later; auto 1 using to_of_val. iNext.
+    iApply wbwp_pure_step_later; auto 1 using to_of_val. iNext; iIntros "_".
     asimpl. change (Rec _) with (of_val (RecV e.[upn 2 (env_subst vs)])) at 2.
-    iApply ("IH" $! Δ (_ :: w :: vs)); last done.
+    iApply ("IH" $! Δ (_ :: w :: vs)).
     iApply interp_env_cons; iSplit; [|iApply interp_env_cons]; auto.
   Qed.
 
   Lemma sem_typed_lam Γ e τ1 τ2 : τ1 :: Γ ⊨ e : τ2 -∗ Γ ⊨ Lam e : TArrow τ1 τ2.
   Proof.
     iIntros "#IH" (Δ vs) "!# #HΓ"; simpl.
-    iIntros (?) "?".
-    iApply wp_value. simpl.
-    iExists _; iFrame; iSplit; last done.
-    iModIntro. iIntros (M' w) "Hreg #Hw".
+    iApply wbwp_value. simpl.
+    iModIntro. iIntros (w) "#Hw".
     iDestruct (interp_env_length with "HΓ") as %?.
-    iApply wp_pure_step_later; auto 1 using to_of_val. iNext.
+    iApply wbwp_pure_step_later; auto 1 using to_of_val. iNext; iIntros "_".
     asimpl.
     iApply ("IH" $! Δ (w :: vs)); auto.
     iApply interp_env_cons; iSplit; auto.
   Qed.
 
-  Lemma sem_typed_letin Γ e1 e2 τ1 τ2 :
-    Γ ⊨ e1 : τ1 -∗ τ1 :: Γ ⊨ e2 : τ2 -∗ Γ ⊨ LetIn e1 e2: τ2.
+  Lemma sem_typed_letin Γ e1 e2 τ1 τ2 : Γ ⊨ e1 : τ1 -∗ τ1 :: Γ ⊨ e2 : τ2 -∗ Γ ⊨ LetIn e1 e2: τ2.
   Proof.
     iIntros "#IH1 #IH2" (Δ vs) "!# #HΓ"; simpl.
-    iIntros (?) "?".
-    smart_wp_bind (LetInCtx _) v "Hv" "IH1"; cbn.
-    iDestruct "Hv" as (N1) "(#Hv&%&Hreg)".
+    smart_wbwp_bind (LetInCtx _) v "#Hv" "IH1"; cbn.
     iDestruct (interp_env_length with "HΓ") as %?.
-    iApply wp_pure_step_later; auto 1 using to_of_val. iNext.
+    iApply wbwp_pure_step_later; auto 1 using to_of_val. iNext; iIntros "_".
     asimpl.
-    iApply (wp_wand with "[Hreg]");
-      first iApply ("IH2" $! Δ (v :: vs) with "[] Hreg");
-      first by iApply interp_env_cons; iSplit; eauto.
-    iIntros (w). iDestruct 1 as (N2) "(?&%&?)".
-    iExists _; iFrame.
-    iPureIntro; etrans; done.
+    iApply ("IH2" $! Δ (v :: vs) with "[]").
+    iApply interp_env_cons; iSplit; eauto.
   Qed.
 
-  Lemma sem_typed_seq Γ e1 e2 τ1 τ2 :
-    Γ ⊨ e1 : τ1 -∗ Γ ⊨ e2 : τ2 -∗ Γ ⊨ Seq e1 e2 : τ2.
+  Lemma sem_typed_seq Γ e1 e2 τ1 τ2 : Γ ⊨ e1 : τ1 -∗ Γ ⊨ e2 : τ2 -∗ Γ ⊨ Seq e1 e2 : τ2.
   Proof.
     iIntros "#IH1 #IH2" (Δ vs) "!# #HΓ"; simpl.
-    iIntros (?) "?".
-    smart_wp_bind (SeqCtx _) v "Hv" "IH1"; cbn.
-    iDestruct "Hv" as (N1) "(#Hv&%&Hreg)".
-    iApply wp_pure_step_later; auto 1 using to_of_val. iNext.
-    iApply (wp_wand with "[Hreg]"); first
-      iApply ("IH2" with "[] Hreg"); first done.
-    iIntros (w). iDestruct 1 as (N2) "(?&%&?)".
-    iExists _; iFrame.
-    iPureIntro; etrans; done.
+    smart_wbwp_bind (SeqCtx _) v "#Hv" "IH1"; cbn.
+    iApply wbwp_pure_step_later; auto 1 using to_of_val. iNext; iIntros "_".
+    iApply ("IH2" with "[]"); first done.
   Qed.
 
-  Lemma sem_typed_app Γ e1 e2 τ1 τ2 :
-      Γ ⊨ e1 : TArrow τ1 τ2 -∗ Γ ⊨ e2 : τ1 -∗ Γ ⊨ App e1 e2 :  τ2.
+  Lemma sem_typed_app Γ e1 e2 τ1 τ2 : Γ ⊨ e1 : TArrow τ1 τ2 -∗ Γ ⊨ e2 : τ1 -∗ Γ ⊨ App e1 e2 :  τ2.
   Proof.
     iIntros "#IH1 #IH2" (Δ vs) "!# #HΓ"; simpl.
-    iIntros (?) "?".
-    smart_wp_bind (AppLCtx (e2.[env_subst vs])) v "Hv" "IH1".
-    iDestruct "Hv" as (N1) "(#Hv&%&Hreg)".
-    smart_wp_bind (AppRCtx v) w "Hw" "IH2".
-    iDestruct "Hw" as (N2) "(#Hw&%&Hreg)".
-    iApply (wp_wand with "[Hreg]"); first
-      iApply ("Hv" with "Hreg"); first done.
-    iIntros (w'). iDestruct 1 as (N3) "(?&%&?)".
-    iExists _; iFrame.
-    iPureIntro; etrans; first etrans; done.
+    smart_wbwp_bind (AppLCtx (e2.[env_subst vs])) v "#Hv" "IH1".
+    smart_wbwp_bind (AppRCtx v) w "Hw" "IH2".
+    iApply "Hv"; done.
   Qed.
 
   Lemma sem_typed_tlam Γ e τ :
     (subst (ren (+1)) <$> Γ) ⊨ e : τ -∗ Γ ⊨ TLam e : TForall τ.
   Proof.
     iIntros "#IH" (Δ vs) "!# #HΓ /=".
-    iIntros (?) "?".
-    iApply wp_value; simpl.
-    iExists _; iFrame; iSplit; last done.
-    iModIntro; iIntros (M' τi) "Hreg".
-    iApply wp_pure_step_later; auto; iNext.
-    iApply "IH"; last done. by iApply interp_env_ren.
+    iApply wbwp_value; simpl.
+    iModIntro; iIntros (τi).
+    iApply wbwp_pure_step_later; auto; iNext; iIntros "_".
+    iApply "IH"; by iApply interp_env_ren.
   Qed.
 
   Lemma sem_typed_tapp Γ e τ τ' : Γ ⊨ e : TForall τ -∗ Γ ⊨ TApp e : τ.[τ'/].
   Proof.
     iIntros "#IH" (Δ vs) "!# #HΓ /=".
-    iIntros (?) "?".
-    smart_wp_bind TAppCtx v "Hv" "IH"; cbn.
-    iDestruct "Hv" as (N1) "(#Hv&%&Hreg)".
-    iApply wp_wand_r; iSplitL;
-      first by iApply ("Hv" $! _ (⟦ τ' ⟧ Δ)).
-    iIntros (w). iDestruct 1 as (N3) "(?&%&?)".
-    iExists _; iFrame; iSplit; first by iApply interp_subst.
-    iPureIntro; etrans; done.
+    smart_wbwp_bind TAppCtx v "#Hv" "IH"; cbn.
+    iApply wbwp_wand_r; iSplitL;
+      first by iApply ("Hv" $! (⟦ τ' ⟧ Δ)).
+    iIntros (w) "?".
+    iApply interp_subst; done.
   Qed.
 
   Lemma sem_typed_pack Γ e τ τ' : Γ ⊨ e : τ.[τ'/] -∗ Γ ⊨ Pack e : TExist τ.
   Proof.
     iIntros "#IH" (Δ vs) "!##HΓ /=".
-    iIntros (?) "?".
-    smart_wp_bind PackCtx v "Hv" "IH".
-    iDestruct "Hv" as (N1) "(#Hv&%&Hreg)".
-    iApply wp_value.
+    smart_wbwp_bind PackCtx v "#Hv" "IH".
+    iApply wbwp_value.
     rewrite -interp_subst.
-    iExists _; iFrame; iSplit; last done.
     iModIntro. iExists (interp _ Δ), _; iSplit; done.
   Qed.
 
@@ -296,29 +206,22 @@ Section typed_interp.
     Γ ⊨ UnpackIn e1 e2 : τ'.
   Proof.
     iIntros "#IH1 #IH2" (Δ vs) "!# #HΓ /=".
-    iIntros (?) "?".
-    smart_wp_bind (UnpackInCtx _) v "Hv" "IH1".
-    iDestruct "Hv" as (N1) "(#Hv&%&Hreg)".
+    smart_wbwp_bind (UnpackInCtx _) v "#Hv" "IH1".
     iDestruct "Hv" as (τi w ->) "#Hw"; simpl.
-    iApply wp_pure_step_later; auto 1 using to_of_val. iNext.
+    iApply wbwp_pure_step_later; auto 1 using to_of_val. iNext; iIntros "_".
     asimpl.
-    iApply wp_wand_r; iSplitL.
-    { iApply ("IH2" $! (τi :: Δ) (w :: vs) with "[] Hreg").
+    iApply wbwp_wand_r; iSplitL.
+    { iApply ("IH2" $! (τi :: Δ) (w :: vs) with "[]").
       iApply interp_env_cons; iSplit; first done.
       iApply interp_env_ren; done. }
-    iIntros (w'). iDestruct 1 as (N3) "(?&%&?)".
-    iExists _; iFrame; iSplit; first by iApply (interp_weaken [] [_]).
-    iPureIntro; etrans; done.
+    iIntros (w') "?". by iApply (interp_weaken [] [_]).
   Qed.
 
   Lemma sem_typed_fold Γ e τ : Γ ⊨ e : τ.[(TRec τ)/] -∗ Γ ⊨ Fold e : TRec τ.
   Proof.
     iIntros "#IH" (Δ vs) "!# #HΓ /=".
-    iIntros (?) "?".
-    smart_wp_bind FoldCtx v "Hv" ("IH" $! Δ vs).
-    iDestruct "Hv" as (N1) "(#Hv&%&Hreg)".
-    iApply wp_value.
-    iExists _; iFrame; iSplit; last done.
+    smart_wbwp_bind FoldCtx v "#Hv" ("IH" $! Δ vs).
+    iApply wbwp_value.
     rewrite /= -interp_subst fixpoint_interp_rec1_eq /=.
     iModIntro; eauto.
   Qed.
@@ -326,44 +229,36 @@ Section typed_interp.
   Lemma sem_typed_unfold Γ e τ : Γ ⊨ e : TRec τ -∗ Γ ⊨ Unfold e : τ.[(TRec τ)/].
   Proof.
     iIntros "#IH" (Δ vs) "!# #HΓ /=".
-    iIntros (?) "?".
-    smart_wp_bind UnfoldCtx v "Hv" ("IH" $! Δ vs).
-    iDestruct "Hv" as (N1) "(#Hv&%&Hreg)".
+    smart_wbwp_bind UnfoldCtx v "#Hv" ("IH" $! Δ vs).
     rewrite /= fixpoint_interp_rec1_eq.
     change (fixpoint _) with (⟦ TRec τ ⟧ Δ); simpl.
     iDestruct "Hv" as (w) "#[% Hw]"; subst.
     simpl.
-    iApply wp_pure_step_later; cbn; auto using to_of_val.
-    iNext. iApply wp_value.
-    iExists _; iFrame; iSplit; last done.
+    iApply wbwp_pure_step_later; cbn; auto using to_of_val.
+    iNext; iIntros "_". iApply wbwp_value.
     by iApply interp_subst.
   Qed.
 
   Lemma sem_typed_alloc Γ e τ : Γ ⊨ e : τ -∗ Γ ⊨ Alloc e : Tref τ.
   Proof.
     iIntros "#IH" (Δ vs) "!# #HΓ /=".
-    iIntros (?) "?".
-    smart_wp_bind AllocCtx v "Hv" "IH"; cbn.
-    iDestruct "Hv" as (N1) "(#Hv&%&Hreg)".
-    iClear "HΓ". iApply wp_fupd.
-    iApply wp_alloc; auto 1 using to_of_val.
+    smart_wbwp_bind AllocCtx v "#Hv" "IH"; cbn.
+    iClear "HΓ". iApply wbwp_fupd.
+    iApply wbwp_alloc; auto 1 using to_of_val.
     iNext; iIntros (l) "Hl".
     iMod (inv_alloc _ _ (∃ v : val, l ↦ᵢ v ∗ ⟦ τ ⟧ Δ v)%I with "[Hl]") as "HN".
     { by iNext; iExists _; iFrame. }
-    iModIntro.
-    iExists _; iFrame; iSplit; [by eauto| done].
+    iModIntro; eauto.
   Qed.
 
   Lemma sem_typed_load Γ e τ : Γ ⊨ e : (Tref τ) -∗ Γ ⊨ Load e : τ.
   Proof.
     iIntros "#IH" (Δ vs) "!# #HΓ /=".
-    iIntros (?) "?".
-    smart_wp_bind LoadCtx v "Hv" "IH"; cbn. iClear "HΓ".
-    iDestruct "Hv" as (N1) "(#Hv&%&Hreg)".
+    smart_wbwp_bind LoadCtx v "#Hv" "IH"; cbn. iClear "HΓ".
     iDestruct "Hv" as (l) "[% #Hv]"; subst.
     iApply wp_atomic.
     iInv (logN .@ l) as (w) "[Hw1 #Hw2]" "Hclose".
-    iApply (wp_load with "Hw1").
+    iApply (wbwp_load with "Hw1").
     iModIntro. iNext.
     iIntros "Hw1". iMod ("Hclose" with "[Hw1 Hw2]"); eauto.
   Qed.
@@ -372,19 +267,15 @@ Section typed_interp.
     Γ ⊨ e1 : (Tref τ) -∗ Γ ⊨ e2 : τ -∗ Γ ⊨ Store e1 e2 : TUnit.
   Proof.
     iIntros "#IH1 #IH2" (Δ vs) "!# #HΓ /=".
-    iIntros (?) "?".
-    smart_wp_bind (StoreLCtx _) v "Hv" "IH1"; cbn.
-    iDestruct "Hv" as (N1) "(#Hv&%&Hreg)".
-    smart_wp_bind (StoreRCtx _) w "Hw" "IH2"; cbn. iClear "HΓ".
-    iDestruct "Hw" as (N2) "(#Hw&%&Hreg)".
+    smart_wbwp_bind (StoreLCtx _) v "#Hv" "IH1"; cbn.
+    smart_wbwp_bind (StoreRCtx _) w "#Hw" "IH2"; cbn. iClear "HΓ".
     iDestruct "Hv" as (l) "[% #Hv]"; subst.
     iApply wp_atomic.
     iInv (logN .@ l) as (z) "[Hz1 #Hz2]" "Hclose".
-    iApply (wp_store with "Hz1"); auto using to_of_val.
+    iApply (wbwp_store with "Hz1"); auto using to_of_val.
     iModIntro. iNext.
     iIntros "Hz1".
     iMod ("Hclose" with "[Hz1 Hz2]") as "_"; first by eauto.
-    iModIntro; iExists _; iFrame; iSplit; first done.
     iPureIntro; etrans; done.
   Qed.
 
