theories/F_mu_ref/unary/soundness.v
@@ -2,38 +2,37 @@ From WBLogrel.F_mu_ref.unary Require Export fundamental.
 From iris.algebra Require Import auth.
 From iris.proofmode Require Import proofmode.
 From iris.program_logic Require Import adequacy.
+From WBLogrel.program_logic Require Import adequacy.
 From iris.prelude Require Import options.
 
 Class soundness_unary_preG Σ := soundness_unary_preIG {
   soundness_unary_preG_iris :> invGpreS Σ;
   soundness_unary_preG_heap :> gen_heapGpreS loc F_mu_ref.val Σ;
-  soundness_unary_preG_reg :> inG Σ (authUR ghost_regUR)
+  soundness_unary_preG_reg :> gstacksGpre Σ
 }.
 
 Theorem soundness Σ `{soundness_unary_preG Σ} e τ e' thp σ σ' :
-  (∀ `{heapIG Σ, ghost_regG Σ}, ⊢ [] ⊨ e : τ) →
+  (∀ `{!heapIG Σ}, ⊢ [] ⊨ e : τ) →
   rtc erased_step ([e], σ) (thp, σ') → e' ∈ thp →
   not_stuck e' σ'.
 Proof.
   intros Hlog ??.
   cut (adequate NotStuck e σ (λ _ _, True));
     first by intros [_ Hsafe]; eapply Hsafe; eauto.
-  eapply (wp_adequacy Σ _). iIntros (Hinv ?).
+  eapply (wbwp_adequacy Σ _). iIntros (Hinv ? ?).
   iMod (gen_heap_init σ) as (Hheap) "[Hh _]".
   iModIntro. iExists (λ σ _, gen_heap_interp σ), (λ _, True%I); iFrame.
-  set (HeapΣ := (HeapIG Σ Hinv Hheap)).
-  iMod ghost_reg_init as (?) "Hreg".
-  iApply (wp_wand with "[Hreg]").
-  - replace e with e.[env_subst[]] by by asimpl.
-    iApply (Hlog HeapΣ $! [] []); [iApply (@interp_env_nil _ HeapΣ)|iFrame].
-  - eauto.
+  set (HeapΣ := (HeapIG Σ Hinv Hheap _)).
+  replace e with e.[env_subst[]] by by asimpl.
+  iApply (wbwp_wand with "[]"); last by iIntros (?) "_".
+  iApply (Hlog HeapΣ $! [] []); iApply (@interp_env_nil _ HeapΣ).
 Qed.
 
 Corollary type_soundness e τ e' thp σ σ' :
   [] ⊢ₜ e : τ →
   rtc erased_step ([e], σ) (thp, σ') → e' ∈ thp → not_stuck e' σ'.
 Proof.
-  intros ??. set (Σ := #[invΣ ; gen_heapΣ loc F_mu_ref.val; ghost_regΣ]).
+  intros ??. set (Σ := #[invΣ ; gen_heapΣ loc F_mu_ref.val; gstacksΣ]).
   set (HG := soundness_unary_preIG Σ _ _ _).
   eapply (soundness Σ); eauto using fundamental.
 Qed.
