theories/program_logic/lifting.v
@@ -1,0 +1,41 @@
+(** This file has been taken from iris and edited accordingly. *)
+(** The "lifting lemmas" in this file serve to lift the rules of the operational
+semantics to the program logic. *)
+
+From iris.proofmode Require Import proofmode.
+From iris.program_logic Require Import lifting.
+From WBLogrel.program_logic Require Export weakestpre.
+From iris.prelude Require Import options.
+
+Section lifting.
+Context `{!irisGS Λ Σ, !gstacksIG Σ}.
+Implicit Types v : val Λ.
+Implicit Types e : expr Λ.
+Implicit Types σ : state Λ.
+Implicit Types P Q : iProp Σ.
+Implicit Types Φ : val Λ → iProp Σ.
+
+Lemma wbwp_pure_step_fupd `{!Inhabited (state Λ)} E E' out e1 e2 φ n Φ :
+  PureExec φ n e1 e2 →
+  φ →
+  (|={E}[E']▷=>^n £ n -∗ WBWP e2 @ out; E {{ Φ }}) ⊢ WBWP e1 @ out; E {{ Φ }}.
+Proof.
+  rewrite /wbwp.
+  iIntros (Hexec Hφ) "Hwp".
+  iIntros (M) "HM".
+  iApply wp_pure_step_fupd; first done.
+  iApply (step_fupdN_wand with "Hwp").
+  iIntros "Hwp H".
+  iSpecialize ("Hwp" with "H HM"); done.
+Qed.
+
+Lemma wbwp_pure_step_later `{!Inhabited (state Λ)} E out e1 e2 φ n Φ :
+  PureExec φ n e1 e2 →
+  φ →
+  ▷^n (£ n -∗ WBWP e2 @ out; E {{ Φ }}) ⊢ WBWP e1 @ out; E {{ Φ }}.
+Proof.
+  intros Hexec ?. rewrite -wbwp_pure_step_fupd //. clear Hexec.
+  enough (∀ P, ▷^n P -∗ |={E}▷=>^n P) as Hwp by apply Hwp. iIntros (?).
+  induction n as [|n IH]; by rewrite //= -step_fupd_intro // IH.
+Qed.
+End lifting.
