theories/program_logic/weakestpre.v
@@ -1,0 +1,490 @@
+(* This file is copied and adapted from the weakestpre file in the iris development. *)
+
+From stdpp Require Export coPset.
+From iris.proofmode Require Import base proofmode classes.
+From iris.base_logic.lib Require Export fancy_updates.
+From iris.program_logic Require Export language.
+From iris.program_logic Require Export weakestpre.
+From WBLogrel Require Export ghost_stacks.
+Import uPred.
+
+Definition wbwp `{!irisGS Λ Σ, !gstacksIG Σ}
+        (E : coPset) (out : gset ghost_id) (e : expr Λ) (Φ : val Λ → iProp Σ) : iProp Σ :=
+  ∀ M, gstacks_except M out -∗ WP e @ E {{v, ∃ N, ⌜M ⊆ N⌝ ∗ gstacks_except N out ∗ Φ v}}.
+
+Global Typeclasses Opaque wbwp.
+
+(** Notations for partial weakest preconditions *)
+(** Notations without binder -- only parsing because they overlap with the
+notations with binder. *)
+Notation "'WBWP' e @ out ; E {{ Φ } }" := (wbwp E out e%E Φ)
+  (at level 20, e, Φ at level 200, only parsing) : bi_scope.
+Notation "'WBWP' e @ E {{ Φ } }" := (wbwp E ∅ e%E Φ)
+  (at level 20, e, Φ at level 200, only parsing) : bi_scope.
+Notation "'WBWP' e {{ Φ } }" := (wbwp ⊤ ∅ e%E Φ)
+  (at level 20, e, Φ at level 200, only parsing) : bi_scope.
+Notation "'WBWP' e '@<' out >{{ Φ } }" := (wbwp ⊤ out e%E Φ)
+  (at level 20, e, Φ at level 200, only parsing) : bi_scope.
+
+Notation "'WBWP' e @ out ; E {{ v , Q } }" := (wbwp E out e%E (λ v, Q))
+  (at level 20, e, Q at level 200,
+   format "'[hv' 'WBWP'  e  '/' @  '[' out ;  '/' E  ']' '/' {{  '[' v ,  '/' Q  ']' } } ']'") : bi_scope.
+Notation "'WBWP' e @ E {{ v , Q } }" := (wbwp E ∅ e%E (λ v, Q))
+  (at level 20, e, Q at level 200,
+   format "'[hv' 'WBWP'  e  '/' @  E  '/' {{  '[' v ,  '/' Q  ']' } } ']'") : bi_scope.
+Notation "'WBWP' e {{ v , Q } }" := (wbwp ⊤ ∅ e%E (λ v, Q))
+  (at level 20, e, Q at level 200,
+   format "'[hv' 'WBWP'  e  '/' {{  '[' v ,  '/' Q  ']' } } ']'") : bi_scope.
+Notation "'WBWP' e '@<' out >{{ v , Q } }" := (wbwp ⊤ out e%E (λ v, Q))
+  (at level 20, e, Q at level 200,
+   format "'[hv' 'WBWP'  e  '/' '@<'  out  >{{  '[' v ,  '/' Q  ']' } } ']'") : bi_scope.
+
+(* Texan triples *)
+Notation "'{WB{{' P } } } e @ out ; E {{{ x .. y , 'RET' pat ; Q } } }" :=
+  (□ ∀ Φ,
+      P -∗ ▷ (∀ x, .. (∀ y, Q -∗ Φ pat%V) .. ) -∗ WBWP e @ out; E {{ Φ }})%I
+    (at level 20, x closed binder, y closed binder,
+     format "'[hv' {WB{{  '[' P  ']' } } }  '/  ' e  '/' @  '[' out ;  '/' E  ']' '/' {{{  '[' x  ..  y ,  RET  pat ;  '/' Q  ']' } } } ']'") : bi_scope.
+Notation "'{WB{{' P } } } e @ E {{{ x .. y , 'RET' pat ; Q } } }" :=
+  (□ ∀ Φ,
+      P -∗ ▷ (∀ x, .. (∀ y, Q -∗ Φ pat%V) .. ) -∗ WBWP e @ E {{ Φ }})%I
+    (at level 20, x closed binder, y closed binder,
+     format "'[hv' {WB{{  '[' P  ']' } } }  '/  ' e  '/' @  E  '/' {{{  '[' x  ..  y ,  RET  pat ;  '/' Q  ']' } } } ']'") : bi_scope.
+Notation "'{WB{{' P } } } e '@<' out >{{{ x .. y , 'RET' pat ; Q } } }" :=
+  (□ ∀ Φ,
+      P -∗ ▷ (∀ x, .. (∀ y, Q -∗ Φ pat%V) .. ) -∗ WBWP e @ out {{ Φ }})%I
+    (at level 20, x closed binder, y closed binder,
+     format "'[hv' {WB{{  '[' P  ']' } } }  '/  ' e  '/' '@<'  out  >{{{  '[' x  ..  y ,  RET  pat ;  '/' Q  ']' } } } ']'") : bi_scope.
+Notation "'{WB{{' P } } } e {{{ x .. y , 'RET' pat ; Q } } }" :=
+  (□ ∀ Φ,
+      P -∗ ▷ (∀ x, .. (∀ y, Q -∗ Φ pat%V) .. ) -∗ WBWP e {{ Φ }})%I
+    (at level 20, x closed binder, y closed binder,
+     format "'[hv' {WB{{  '[' P  ']' } } }  '/  ' e  '/' {{{  '[' x  ..  y ,  RET  pat ;  '/' Q  ']' } } } ']'") : bi_scope.
+
+Notation "'{WB{{' P } } } e @ out ; E {{{ 'RET' pat ; Q } } }" :=
+  (□ ∀ Φ, P -∗ ▷ (Q -∗ Φ pat%V) -∗ WBWP e @ out; E {{ Φ }})%I
+    (at level 20,
+     format "'[hv' {WB{{  '[' P  ']' } } }  '/  ' e  '/' @  '[' out ;  '/' E  ']' '/' {{{  '[' RET  pat ;  '/' Q  ']' } } } ']'") : bi_scope.
+Notation "'{WB{{' P } } } e @ E {{{ 'RET' pat ; Q } } }" :=
+  (□ ∀ Φ, P -∗ ▷ (Q -∗ Φ pat%V) -∗ WBWP e @ E {{ Φ }})%I
+    (at level 20,
+     format "'[hv' {WB{{  '[' P  ']' } } }  '/  ' e  '/' @  E  '/' {{{  '[' RET  pat ;  '/' Q  ']' } } } ']'") : bi_scope.
+Notation "'{WB{{' P } } } e '@<' out >{{{ 'RET' pat ; Q } } }" :=
+  (□ ∀ Φ, P -∗ ▷ (Q -∗ Φ pat%V) -∗ WBWP e @ out {{ Φ }})%I
+    (at level 20,
+     format "'[hv' {WB{{  '[' P  ']' } } }  '/  ' e  '/' '@<'  out  >{{{  '[' RET  pat ;  '/' Q  ']' } } } ']'") : bi_scope.
+Notation "'{WB{{' P } } } e {{{ 'RET' pat ; Q } } }" :=
+  (□ ∀ Φ, P -∗ ▷ (Q -∗ Φ pat%V) -∗ WBWP e {{ Φ }})%I
+    (at level 20,
+     format "'[hv' {WB{{  '[' P  ']' } } }  '/  ' e  '/' {{{  '[' RET  pat ;  '/' Q  ']' } } } ']'") : bi_scope.
+
+(** Aliases for stdpp scope -- they inherit the levels and format from above. *)
+Notation "'{WB{{' P } } } e @ out ; E {{{ x .. y , 'RET' pat ; Q } } }" :=
+  (∀ Φ, P -∗ ▷ (∀ x, .. (∀ y, Q -∗ Φ pat%V) .. ) -∗ WBWP e @ out; E {{ Φ }}) : stdpp_scope.
+Notation "'{WB{{' P } } } e @ E {{{ x .. y , 'RET' pat ; Q } } }" :=
+  (∀ Φ, P -∗ ▷ (∀ x, .. (∀ y, Q -∗ Φ pat%V) .. ) -∗ WBWP e @ E {{ Φ }}) : stdpp_scope.
+Notation "'{WB{{' P } } } e '@<' out >{{{ x .. y , 'RET' pat ; Q } } }" :=
+  (∀ Φ, P -∗ ▷ (∀ x, .. (∀ y, Q -∗ Φ pat%V) .. ) -∗ WBWP e @< out >{{ Φ }}) : stdpp_scope.
+Notation "'{WB{{' P } } } e {{{ x .. y , 'RET' pat ; Q } } }" :=
+  (∀ Φ, P -∗ ▷ (∀ x, .. (∀ y, Q -∗ Φ pat%V) .. ) -∗ WBWP e {{ Φ }}) : stdpp_scope.
+Notation "'{WB{{' P } } } e @ out ; E {{{ 'RET' pat ; Q } } }" :=
+  (∀ Φ, P -∗ ▷ (Q -∗ Φ pat%V) -∗ WBWP e @ out; E {{ Φ }}) : stdpp_scope.
+Notation "'{WB{{' P } } } e @ E {{{ 'RET' pat ; Q } } }" :=
+  (∀ Φ, P -∗ ▷ (Q -∗ Φ pat%V) -∗ WBWP e @ E {{ Φ }}) : stdpp_scope.
+Notation "'{WB{{' P } } } e @< out > {{{ 'RET' pat ; Q } } }" :=
+  (∀ Φ, P -∗ ▷ (Q -∗ Φ pat%V) -∗ WBWP e @< out >{{ Φ }}) : stdpp_scope.
+Notation "'{WB{{' P } } } e {{{ 'RET' pat ; Q } } }" :=
+  (∀ Φ, P -∗ ▷ (Q -∗ Φ pat%V) -∗ WBWP e {{ Φ }}) : stdpp_scope.
+
+Section wp.
+Context `{!irisGS Λ Σ, !gstacksIG Σ}.
+Implicit Types P : iProp Σ.
+Implicit Types Φ : val Λ → iProp Σ.
+Implicit Types v : val Λ.
+Implicit Types e : expr Λ.
+
+Global Instance wbwp_ne E out e n :
+  Proper (pointwise_relation _ (dist n) ==> dist n) (wbwp E out e).
+Proof. intros ???; rewrite /wbwp /=; repeat f_equiv. Qed.
+Global Instance wbwp_proper E out e :
+  Proper (pointwise_relation _ (≡) ==> (≡)) (wbwp E out e).
+Proof.
+  by intros Φ Φ' ?; apply equiv_dist=>n; apply wbwp_ne=>v; apply equiv_dist.
+Qed.
+Global Instance wbwp_contractive E out e n :
+  TCEq (to_val e) None →
+  Proper (pointwise_relation _ (dist_later n) ==> dist n) (wbwp E out e).
+Proof.
+  intros He Φ Ψ HΦ.
+  rewrite /wbwp /=; do 3 f_equiv; apply wp_contractive; first done.
+  f_equiv.
+  destruct n; first done; simpl.
+  repeat f_equiv.
+Qed.
+
+Lemma wbwp_value_fupd' E out Φ v : (|={E}=> Φ v) ⊢ WBWP of_val v @ out; E {{ Φ }}.
+Proof. rewrite /wbwp; iIntros ">?" (?) "?"; iApply wp_value'; iExists _; iFrame; done. Qed.
+
+Lemma wbwp_strong_mono E1 E2 out e Φ Ψ :
+  E1 ⊆ E2 →
+  WBWP e @ out; E1 {{ Φ }} -∗ (∀ v, Φ v ={E2}=∗ Ψ v) -∗ WBWP e @ out; E2 {{ Ψ }}.
+Proof.
+  iIntros (HE) "H HΦ".
+  rewrite /wbwp.
+  iIntros (M) "HM".
+  iApply (wp_strong_mono with "[H HM]"); [done|eassumption|by iApply "H"|].
+  iIntros (?); iDestruct 1 as (?) "[? [? ?]]".
+  iMod ("HΦ" with "[$]").
+  iModIntro; iExists _; iFrame.
+Qed.
+
+Lemma wbwp_get_gstack_full n E out e Φ :
+  n ∉ out →
+  gstack_exists n -∗
+  (∀ s, gstack_full n s -∗ WBWP e @ (out ∪ {[n]}); E {{v, gstack_full n s ∗ Φ v }}) -∗
+  WBWP e @ out; E {{ Φ }}.
+Proof.
+  iIntros (?) "#Hex HWBWP".
+  rewrite /wbwp.
+  iIntros (M) "HM".
+  iDestruct (gstack_exists_in with "Hex HM") as %?.
+  iDestruct (gstacks_take_out _ _ n with "Hex HM") as (s HMn) "[HM Hfl]"; first set_solver.
+  iApply (wp_wand with "[HM Hfl HWBWP]").
+  { iApply ("HWBWP" with "[$] [$]"). }
+  iIntros (?); iDestruct 1 as (N HNM) "(Hgs & Hfl & HΦ)".
+  iDestruct (gstacks_put_back with "Hfl Hgs") as "Hgs"; first by eapply lookup_weaken; eauto.
+  replace ((out ∪ {[n]}) ∖ {[n]}) with out by set_solver.
+  iExists _; iFrame; done.
+Qed.
+
+Lemma wbwp_mend n s E out e Φ :
+  gstack_full n s -∗
+  WBWP e @ out ∖ {[n]}; E {{ Φ }} -∗
+  WBWP e @ out; E {{v, gstack_full n s ∗ Φ v }}.
+Proof.
+  iIntros "Hfl HWBWP".
+  rewrite /wbwp.
+  iIntros (M) "HM".
+  iDestruct (gstack_full_is_out with "Hfl HM") as %?.
+  iDestruct (gstacks_except_included with "HM") as "%".
+  iDestruct (gstack_full_exists with "Hfl") as "#Hex".
+  destruct (M !! n) as [s'|] eqn:HMns'; last by apply not_elem_of_dom in HMns'; set_solver.
+  iDestruct (gstacks_out_swap _ _ n s with "HM") as "HM"; first done.
+  iDestruct (gstacks_put_back with "Hfl HM") as "HM"; first by rewrite lookup_insert.
+  iSpecialize ("HWBWP" with "HM").
+  iApply (wp_wand with "[$]").
+  iIntros (?); iDestruct 1 as (N) "(%&HM&?)".
+  iDestruct (gstacks_take_out _ _ n with "Hex HM") as (s'' HMn) "[HM Hfl]"; first set_solver.
+  replace (out ∖ {[n]} ∪ {[n]}) with out; last first.
+  { apply set_eq; intros m; split; [|set_solver]. destruct (decide (n = m)); set_solver. }
+  iDestruct (gstacks_out_swap _ _ n s' with "HM") as "HM"; first done.
+  assert (N !! n = Some s).
+  { eapply lookup_weaken; last eassumption. rewrite lookup_insert //. }
+  simplify_eq /=.
+  iExists _; iFrame.
+  iPureIntro.
+  apply map_subseteq_spec.
+  intros i ? HMi.
+  destruct (decide (i = n)) as [->|]; first by rewrite HMns' in HMi; rewrite lookup_insert.
+  rewrite lookup_insert_ne //.
+  eapply lookup_weaken; last eassumption.
+  rewrite lookup_insert_ne //.
+Qed.
+
+Lemma wbwp_make_gstack E out γ e Φ :
+  (∀ n, gstack_frag n (gsingleton γ) -∗ WBWP e @ out; E {{ Φ }}) -∗ WBWP e @ out; E {{ Φ }}.
+Proof.
+  iIntros "HWBWP".
+  rewrite /wbwp.
+  iIntros (M) "HM".
+  iMod (gstack_alloc _ _ γ with "HM") as (n) "(%&HM&Hfr)".
+  iApply (wp_wand with "[HM Hfr HWBWP]"); first by iApply ("HWBWP" with "[$] [$]").
+  iIntros (?); iDestruct 1 as (N HNM) "(Hgs & HΦ)".
+  iExists _; iFrame.
+  iPureIntro.
+  etrans; last eassumption.
+  apply insert_subseteq, not_elem_of_dom; done.
+Qed.
+
+Lemma fupd_wbwp E out e Φ : (|={E}=> WBWP e @ out; E {{ Φ }}) ⊢ WBWP e @ out; E {{ Φ }}.
+Proof. rewrite /wbwp; iIntros "H" (M) "?"; iMod "H"; iApply "H"; iAssumption. Qed.
+Lemma wbwp_fupd E out e Φ : WBWP e @ out; E {{ v, |={E}=> Φ v }} ⊢ WBWP e @ out; E {{ Φ }}.
+Proof. iIntros "H". iApply (wbwp_strong_mono E with "H"); auto. Qed.
+
+Lemma wp_atomic E1 E2 out e Φ `{!Atomic WeaklyAtomic e} :
+  (|={E1,E2}=> WBWP e @ out; E2 {{ v, |={E2,E1}=> Φ v }}) ⊢ WBWP e @ out; E1 {{ Φ }}.
+Proof.
+  rewrite /wbwp; iIntros "H" (M) "HM".
+  iApply wp_atomic.
+  iMod "H"; iModIntro.
+  iApply (wp_wand with "[H HM]"); first by iApply "H".
+  iIntros (?); iDestruct 1 as (?) "(?&?&>?)".
+  iModIntro; iExists _; iFrame.
+Qed.
+
+Lemma wp_wbwp E out e Φ : WP e @ E {{ Φ }} -∗ WBWP e @ out; E {{ Φ }}.
+Proof.
+  iIntros "HWP".
+  rewrite /wbwp.
+  iIntros (M) "HM".
+  iApply (wp_wand with "HWP").
+  iIntros (?) "?"; iExists _; iFrame; done.
+Qed.
+
+(** This lemma gives us access to the later credits that are generated in each step,
+  assuming that we have instantiated [num_laters_per_step] with a non-trivial (e.g. linear)
+  function.
+  This lemma can be used to provide a "regeneration" mechanism for later credits.
+  [state_interp] will have to be defined in a way that involves the required regneration
+  tokens. TODO: point to an example of how this is used.
+
+  In detail, a client can use this lemma as follows:
+  * the client obtains the state interpretation [state_interp _ ns _ _],
+  * it uses some ghost state wired up to the interpretation to know that
+    [ns = k + m], and update the state interpretation to [state_interp _ m _ _],
+  * _after_ [e] has finally stepped, we get [num_laters_per_step k] later credits
+    that we can use to prove [P] in the postcondition, and we have to update
+    the state interpretation from [state_interp _ (S m) _ _] to
+    [state_interp _ (S ns) _ _] again. *)
+Lemma wbwp_credit_access E out e Φ P :
+  TCEq (to_val e) None →
+  (∀ m k, num_laters_per_step m + num_laters_per_step k ≤ num_laters_per_step (m + k)) →
+  (∀ σ1 ns κs nt, state_interp σ1 ns κs nt ={E}=∗
+    ∃ k m, state_interp σ1 m κs nt ∗ ⌜ns = (m + k)%nat⌝ ∗
+    (∀ nt σ2 κs, £ (num_laters_per_step k) -∗ state_interp σ2 (S m) κs nt ={E}=∗
+      state_interp σ2 (S ns) κs nt ∗ P)) -∗
+  WBWP e @ out; E {{ v, P ={E}=∗ Φ v }} -∗
+  WBWP e @ out; E {{ Φ }}.
+Proof.
+  rewrite /wbwp.
+  iIntros (? ?) "Hupd Hwp".
+  iIntros (M) "HM".
+  iApply (wp_credit_access with "Hupd"); first done.
+  iApply (wp_wand with "[Hwp HM]"); first by iApply "Hwp".
+  iIntros (?); iDestruct 1 as (?) "(?&?&H)".
+  iIntros "HP"; iMod ("H" with "HP").
+  iModIntro; iExists _; iFrame.
+Qed.
+
+(** In this stronger version of [wp_step_fupdN], the masks in the
+   step-taking fancy update are a bit weird and somewhat difficult to
+   use in practice. Hence, we prove it for the sake of completeness,
+   but [wp_step_fupdN] is just a little bit weaker, suffices in
+   practice and is easier to use.
+
+   See the statement of [wp_step_fupdN] below to understand the use of
+   ordinary conjunction here. *)
+Lemma wbwp_step_fupdN_strong k E1 E2 out e P Φ :
+  TCEq (to_val e) None → E2 ⊆ E1 →
+  (∀ σ ns κs nt, state_interp σ ns κs nt
+       ={E1,∅}=∗ ⌜k ≤ S (num_laters_per_step ns)⌝) ∧
+  ((|={E1,E2}=> |={∅}▷=>^k |={E2,E1}=> P) ∗
+    WBWP e @ out; E2 {{ v, P ={E1}=∗ Φ v }}) -∗
+  WBWP e @ out; E1 {{ Φ }}.
+Proof.
+  rewrite /wbwp.
+  iIntros (? ?) "Hwp".
+  iIntros (M) "HM".
+  iApply (wp_step_fupdN_strong); first done.
+  iSplit; first iDestruct "Hwp" as "[$ _]".
+  iDestruct "Hwp" as "[_ [$ Hwp]]".
+  iApply (wp_wand with "[Hwp HM]"); first by iApply "Hwp".
+  iIntros (?); iDestruct 1 as (?) "(?&?&H)".
+  iIntros "HP"; iMod ("H" with "HP").
+  iModIntro; iExists _; iFrame.
+Qed.
+
+Lemma wbwp_bind K `{!LanguageCtx K} E out e Φ :
+  WBWP e @ out; E {{ v, WBWP K (of_val v) @ out; E {{ Φ }} }} ⊢ WBWP K e @ out; E {{ Φ }}.
+Proof.
+  rewrite /wbwp.
+  iIntros "Hwp" (M) "HM".
+  iApply wp_bind.
+  iApply (wp_wand with "[Hwp HM]"); first by iApply "Hwp".
+  iIntros (?); iDestruct 1 as (?) "(%&HM&Hwp)".
+  iApply (wp_wand with "[Hwp HM]"); first by iApply "Hwp".
+  iIntros (?); iDestruct 1 as (?) "(%&HM&Hwp)".
+  iExists _; iFrame; iPureIntro.
+  etrans; eauto.
+Qed.
+
+(* The following lemma does not work for well-bracketed weakest preconditions. *)
+(* The reason is that it could be that the stack is broken across evaluation context and is only *)
+(* going to be mended afterwards. *)
+(* Lemma wbwp_bind_inv K `{!LanguageCtx K} E out e Φ : *)
+(*   WBWP K e @ out; E {{ Φ }} ⊢ WBWP e @ out; E {{ v, WBWP K (of_val v) @ out; E {{ Φ }} }}. *)
+
+(** * Derived rules *)
+Lemma wbwp_mono E out e Φ Ψ : (∀ v, Φ v ⊢ Ψ v) → WBWP e @ out; E {{ Φ }} ⊢ WBWP e @ out; E {{ Ψ }}.
+Proof.
+  iIntros (HΦ) "H"; iApply (wbwp_strong_mono with "H"); auto.
+  iIntros (v) "?". by iApply HΦ.
+Qed.
+(* Lemma wp_stuck_mono s1 s2 E e Φ : *)
+(*   s1 ⊑ s2 → WP e @ s1; E {{ Φ }} ⊢ WP e @ s2; E {{ Φ }}. *)
+(* Proof. iIntros (?) "H". iApply (wp_strong_mono with "H"); auto. Qed. *)
+(* Lemma wp_stuck_weaken s E e Φ : *)
+(*   WP e @ s; E {{ Φ }} ⊢ WP e @ E ?{{ Φ }}. *)
+(* Proof. apply wp_stuck_mono. by destruct s. Qed. *)
+Lemma wb_mask_mono E1 E2 out e Φ : E1 ⊆ E2 → WBWP e @ out; E1 {{ Φ }} ⊢ WBWP e @ out; E2 {{ Φ }}.
+Proof. iIntros (?) "H"; iApply (wbwp_strong_mono with "H"); auto. Qed.
+Global Instance wbwp_mono' E out e :
+  Proper (pointwise_relation _ (⊢) ==> (⊢)) (wbwp E out e).
+Proof. by intros Φ Φ' ?; apply wbwp_mono. Qed.
+Global Instance wbwp_flip_mono' E out e :
+  Proper (pointwise_relation _ (flip (⊢)) ==> (flip (⊢))) (wbwp E out e).
+Proof. by intros Φ Φ' ?; apply wbwp_mono. Qed.
+
+Lemma wbwp_value_fupd s E Φ e v : IntoVal e v → (|={E}=> Φ v) -∗ WBWP e @ s; E {{ Φ }}.
+Proof. intros <-. by apply wbwp_value_fupd'. Qed.
+Lemma wbwp_value' E out Φ v : Φ v ⊢ WBWP (of_val v) @ out; E {{ Φ }}.
+Proof. rewrite -wbwp_value_fupd'; auto. Qed.
+Lemma wbwp_value E out Φ e v : IntoVal e v → Φ v ⊢ WBWP e @ out; E {{ Φ }}.
+Proof. intros <-. apply wbwp_value'. Qed.
+
+Lemma wbwp_frame_l E out e Φ R : R ∗ WBWP e @ out; E {{ Φ }} ⊢ WBWP e @ out; E {{ v, R ∗ Φ v }}.
+Proof. iIntros "[? H]". iApply (wbwp_strong_mono with "H"); auto with iFrame. Qed.
+Lemma wbwp_frame_r E out e Φ R : WBWP e @ out; E {{ Φ }} ∗ R ⊢ WBWP e @ out; E {{ v, Φ v ∗ R }}.
+Proof. iIntros "[H ?]". iApply (wbwp_strong_mono with "H"); auto with iFrame. Qed.
+
+(** This lemma states that if we can prove that [n] laters are used in
+   the current physical step, then one can perform an n-steps fancy
+   update during that physical step. The resources needed to prove the
+   bound on [n] are not used up: they can be reused in the proof of
+   the WP or in the proof of the n-steps fancy update. In order to
+   describe this unusual resource flow, we use ordinary conjunction as
+   a premise. *)
+Lemma wbwp_step_fupdN n E1 E2 out e P Φ :
+  TCEq (to_val e) None → E2 ⊆ E1 →
+  (∀ σ ns κs nt, state_interp σ ns κs nt
+       ={E1,∅}=∗ ⌜n ≤ S (num_laters_per_step ns)⌝) ∧
+  ((|={E1∖E2,∅}=> |={∅}▷=>^n |={∅,E1∖E2}=> P) ∗
+    WBWP e @ out; E2 {{ v, P ={E1}=∗ Φ v }}) -∗
+  WBWP e @ out; E1 {{ Φ }}.
+Proof.
+  iIntros (??) "H". iApply (wbwp_step_fupdN_strong with "[H]"); [done|].
+  iApply (and_mono_r with "H"). apply sep_mono_l. iIntros "HP".
+  iMod fupd_mask_subseteq_emptyset_difference as "H"; [|iMod "HP"]; [set_solver|].
+  iMod "H" as "_". replace (E1 ∖ (E1 ∖ E2)) with E2; last first.
+  { set_unfold=>x. destruct (decide (x ∈ E2)); naive_solver. }
+  iModIntro. iApply (step_fupdN_wand with "HP"). iIntros "H".
+  iApply fupd_mask_frame; [|iMod "H"; iModIntro]; [set_solver|].
+  by rewrite difference_empty_L (comm_L (∪)) -union_difference_L.
+Qed.
+Lemma wbwp_step_fupd E1 E2 out e P Φ :
+  TCEq (to_val e) None → E2 ⊆ E1 →
+  (|={E1}[E2]▷=> P) -∗ WBWP e @ out; E2 {{ v, P ={E1}=∗ Φ v }} -∗ WBWP e @ out; E1 {{ Φ }}.
+Proof.
+  iIntros (??) "HR H".
+  iApply (wbwp_step_fupdN_strong 1 E1 E2 with "[-]"); [done|..]. iSplit.
+  - iIntros (????) "_". iMod (fupd_mask_subseteq ∅) as "_"; [set_solver+|].
+    auto with lia.
+  - iFrame "H". iMod "HR" as "$". auto.
+Qed.
+
+Lemma wbwp_frame_step_l E1 E2 out e Φ R :
+  TCEq (to_val e) None → E2 ⊆ E1 →
+  (|={E1}[E2]▷=> R) ∗ WBWP e @ out; E2 {{ Φ }} ⊢ WBWP e @ out; E1 {{ v, R ∗ Φ v }}.
+Proof.
+  iIntros (??) "[Hu Hwp]". iApply (wbwp_step_fupd with "Hu"); try done.
+  iApply (wbwp_mono with "Hwp"). by iIntros (?) "$$".
+Qed.
+Lemma wbwp_frame_step_r E1 E2 out e Φ R :
+  TCEq (to_val e) None → E2 ⊆ E1 →
+  WBWP e @ out; E2 {{ Φ }} ∗ (|={E1}[E2]▷=> R) ⊢ WBWP e @ out; E1 {{ v, Φ v ∗ R }}.
+Proof.
+  rewrite [(WBWP _ @ _; _ {{ _ }} ∗ _)%I]comm; setoid_rewrite (comm _ _ R).
+  apply wbwp_frame_step_l.
+Qed.
+Lemma wbwp_frame_step_l' E out e Φ R :
+  TCEq (to_val e) None → ▷ R ∗ WBWP e @ out; E {{ Φ }} ⊢ WBWP e @ out; E {{ v, R ∗ Φ v }}.
+Proof. iIntros (?) "[??]". iApply (wbwp_frame_step_l E E); try iFrame; eauto. Qed.
+Lemma wbwp_frame_step_r' E out e Φ R :
+  TCEq (to_val e) None → WBWP e @ out; E {{ Φ }} ∗ ▷ R ⊢ WBWP e @ out; E {{ v, Φ v ∗ R }}.
+Proof. iIntros (?) "[??]". iApply (wbwp_frame_step_r E E out); try iFrame; eauto. Qed.
+
+Lemma wbwp_wand E out e Φ Ψ :
+  WBWP e @ out; E {{ Φ }} -∗ (∀ v, Φ v -∗ Ψ v) -∗ WBWP e @ out; E {{ Ψ }}.
+Proof.
+  iIntros "Hwp H". iApply (wbwp_strong_mono with "Hwp"); auto.
+  iIntros (?) "?". by iApply "H".
+Qed.
+Lemma wbwp_wand_l E out e Φ Ψ :
+  (∀ v, Φ v -∗ Ψ v) ∗ WBWP e @ out; E {{ Φ }} ⊢ WBWP e @ out; E {{ Ψ }}.
+Proof. iIntros "[H Hwp]". iApply (wbwp_wand with "Hwp H"). Qed.
+Lemma wbwp_wand_r E out e Φ Ψ :
+  WBWP e @ out; E {{ Φ }} ∗ (∀ v, Φ v -∗ Ψ v) ⊢ WBWP e @ out; E {{ Ψ }}.
+Proof. iIntros "[Hwp H]". iApply (wbwp_wand with "Hwp H"). Qed.
+Lemma wp_frame_wand E out e Φ R :
+  R -∗ WBWP e @ out; E {{ v, R -∗ Φ v }} -∗ WBWP e @ out; E {{ Φ }}.
+Proof.
+  iIntros "HR HWP". iApply (wbwp_wand with "HWP").
+  iIntros (v) "HΦ". by iApply "HΦ".
+Qed.
+End wp.
+
+(** Proofmode class instances *)
+Section proofmode_classes.
+  Context `{!irisGS Λ Σ, !gstacksIG Σ}.
+  Implicit Types P Q : iProp Σ.
+  Implicit Types Φ : val Λ → iProp Σ.
+  Implicit Types v : val Λ.
+  Implicit Types e : expr Λ.
+
+  Global Instance frame_wbwp p E out e R Φ Ψ :
+    (∀ v, Frame p R (Φ v) (Ψ v)) →
+    Frame p R (WBWP e @ out; E {{ Φ }}) (WBWP e @ out; E {{ Ψ }}) | 2.
+  Proof. rewrite /Frame=> HR. rewrite wbwp_frame_l. apply wbwp_mono, HR. Qed.
+
+  Global Instance is_except_0_wbwp E out e Φ : IsExcept0 (WBWP e @ out; E {{ Φ }}).
+  Proof. by rewrite /IsExcept0 -{2}fupd_wbwp -except_0_fupd -fupd_intro. Qed.
+
+  Global Instance elim_modal_bupd_wbwp p E out e P Φ :
+    ElimModal True p false (|==> P) P (WBWP e @ out; E {{ Φ }}) (WBWP e @ out; E {{ Φ }}).
+  Proof.
+    by rewrite /ElimModal intuitionistically_if_elim
+      (bupd_fupd E) fupd_frame_r wand_elim_r fupd_wbwp.
+  Qed.
+
+  Global Instance elim_modal_fupd_wbwp p E out e P Φ :
+    ElimModal True p false (|={E}=> P) P (WBWP e @ out; E {{ Φ }}) (WBWP e @ out; E {{ Φ }}).
+  Proof.
+    by rewrite /ElimModal intuitionistically_if_elim
+      fupd_frame_r wand_elim_r fupd_wbwp.
+  Qed.
+
+  Global Instance elim_modal_fupd_wbwp_atomic p E1 E2 out e P Φ :
+    ElimModal (Atomic WeaklyAtomic e) p false
+            (|={E1,E2}=> P) P
+            (WBWP e @ out; E1 {{ Φ }}) (WBWP e @ out; E2 {{ v, |={E2,E1}=> Φ v }})%I | 100.
+  Proof.
+    intros ?. by rewrite intuitionistically_if_elim
+      fupd_frame_r wand_elim_r wp_atomic.
+  Qed.
+
+  Global Instance add_modal_fupd_wbwp E out e P Φ :
+    AddModal (|={E}=> P) P (WBWP e @ out; E {{ Φ }}).
+  Proof. by rewrite /AddModal fupd_frame_r wand_elim_r fupd_wbwp. Qed.
+
+  Global Instance elim_acc_wbwp_atomic {X} E1 E2 α β γ out e Φ :
+    ElimAcc (X:=X) (Atomic WeaklyAtomic e)
+            (fupd E1 E2) (fupd E2 E1)
+            α β γ (WBWP e @ out; E1 {{ Φ }})
+            (λ x, WBWP e @ out; E2 {{ v, |={E2}=> β x ∗ (γ x -∗? Φ v) }})%I | 100.
+  Proof.
+    iIntros (?) "Hinner >Hacc". iDestruct "Hacc" as (x) "[Hα Hclose]".
+    iApply (wbwp_wand with "(Hinner Hα)").
+    iIntros (v) ">[Hβ HΦ]". iApply "HΦ". by iApply "Hclose".
+  Qed.
+
+  Global Instance elim_acc_wbwp_nonatomic {X} E α β γ out e Φ :
+    ElimAcc (X:=X) True (fupd E E) (fupd E E)
+            α β γ (WBWP e @ out; E {{ Φ }})
+            (λ x, WBWP e @ out; E {{ v, |={E}=> β x ∗ (γ x -∗? Φ v) }})%I.
+  Proof.
+    iIntros (_) "Hinner >Hacc". iDestruct "Hacc" as (x) "[Hα Hclose]".
+    iApply wbwp_fupd.
+    iApply (wbwp_wand with "(Hinner Hα)").
+    iIntros (v) ">[Hβ HΦ]". iApply "HΦ". by iApply "Hclose".
+  Qed.
+End proofmode_classes.
